examples/lowparse/LowParse.Impl.VLBytes.Part1.fst
@@ -13,23 +13,75 @@ module HST = FStar.HyperStack.ST
 module E = FStar.Kremlin.Endianness
 module Cast = FStar.Int.Cast
 
-#set-options "--z3rlimit 64"
-
-let parse_bounded_vlbytes_parse_vlbytes
+val parse_bounded_vlbytes_parse_vlbytes
   (min: U32.t)
   (max: U32.t { U32.v max > 0 } )
-  (#b: bool)
+  (#k: parser_kind)
   (#t: Type0)
   (h: HS.mem)
-  (p: parser' b t)
+  (p: parser k t)
   (b: S.bslice)
   (pred: ((t * consumed_slice_length b) -> GTot Type0))
 : Lemma
   (requires (parses h (parse_bounded_vlbytes min max p) b pred))
   (ensures (parses h (parse_vlbytes (log256 max) p) b pred))
-= ()
 
-#reset-options
+#set-options "--z3rlimit 128 --max_fuel 8 --max_ifuel 8"
+
+let parse_bounded_vlbytes_parse_vlbytes min max #k #t h p b pred =
+  let s = S.as_seq h b in
+  let sz = log256 max in
+  let f = in_bounds min max in
+  assert (Some? (parse (parse_vlbytes_gen sz f p) s));
+  parse_flbytes_and_then_cases_injective sz f p;
+  assert (Some? (parse (
+    (parse_filter (parse_bounded_integer sz) f)
+    `and_then`
+    (parse_vlbytes_payload sz f p)
+  ) s));
+  assert (Some? (parse (parse_filter (parse_bounded_integer sz) f) s));
+  let (Some (len1, sz1)) = parse (parse_filter (parse_bounded_integer sz) f) s in
+  assert (Some? (parse (parse_bounded_integer sz) s));
+  let (Some (len2, sz2)) = parse (parse_bounded_integer sz) s in
+  assert (sz1 == sz2);
+  assert ((len1 <: bounded_integer sz) == len2);
+  let pv1: bare_parser t = parse_vlbytes_payload sz f p len1 in
+  let s'1 : bytes32 = Seq.slice s sz1 (Seq.length s) in
+  let s'2 : bytes32 = Seq.slice s sz2 (Seq.length s) in
+  assert (s'1 == s'2);
+  assert (Some? (parse pv1 s'1));
+  let (Some (v1, consumed1)) = parse pv1 s'1 in
+  let pv2: bare_parser t = parse_vlbytes_payload sz f p len2 in
+  assert (Some? (parse pv2 s'2));
+  let (Some (v2, consumed2)) = parse pv2 s'2 in
+  assert (v1 == v2);
+  assert ((consumed1 <: nat) == (consumed2 <: nat));
+  let total1: consumed_slice_length b = U32.uint_to_t (sz1 + consumed1) in
+  let total2: consumed_slice_length b = U32.uint_to_t (sz2 + consumed2) in
+  assert (total1 == total2);
+  assert (pred (v1, total1));
+  assert (pred (v2, total2))
+
+(*
+  let (Some (len, sz')) = parse (parse_bounded_integer sz) s in
+  assert ((sz' <: nat) == (sz <: nat));
+  assert (in_bounds min max len);
+  let len_ : (i: bounded_integer sz { in_bounds min max i == true } ) = len in
+  let p' : bare_parser t = parse_vlbytes_payload sz (in_bounds min max) p len_ in
+  let sz' : nat = sz' in
+  let s' : bytes32 = Seq.slice s sz' (Seq.length s) in
+  assert (Some? (parse (parse_filter (parse_bounded_integer sz) (in_bounds min max)) s));
+  let (Some (len', sz'')) = parse (parse_filter (parse_bounded_integer sz) (in_bounds min max)) s in
+  let len' : bounded_integer sz = len' in
+  assert (len == len');
+  assert (Some? (parse p' s'));
+  admit ()
+
+(*  
+  assert (Some? (parse (parse_flbytes p (U32.v len)) s'));
+  let (Some (v, len')) = parse (parse_flbytes p (U32.v len)) s' in
+  assert (len' == U32.v len);
+  admit ()
 
 inline_for_extraction
 let parse_bounded_integer_1_synth
@@ -38,7 +90,7 @@ let parse_bounded_integer_1_synth
 = Cast.uint8_to_uint32 x
 
 let parse_bounded_integer_1
-: parser (bounded_integer 1)
+: parser _ (bounded_integer 1)
 = parse_synth parse_u8 parse_bounded_integer_1_synth
 
 inline_for_extraction
@@ -48,7 +100,7 @@ let parse_bounded_integer_2_synth
 = Cast.uint16_to_uint32 x
 
 let parse_bounded_integer_2
-: parser (bounded_integer 2)
+: parser _ (bounded_integer 2)
 = parse_synth parse_u16 parse_bounded_integer_2_synth
 
 #set-options "--z3rlimit 32"
@@ -63,15 +115,19 @@ let parse_bounded_integer_3_synth
 #reset-options
 
 let parse_bounded_integer_3
-: parser (bounded_integer 3)
+: parser _ (bounded_integer 3)
 = (parse_u16 `nondep_then` parse_u8) `parse_synth` parse_bounded_integer_3_synth
 
 val parse_bounded_integer'
   (i: integer_size)
-: parser (bounded_integer i)
+: parser (ParserStrong (StrongConstantSize i ConstantSizeTotal)) (bounded_integer i)
 
-let parse_bounded_integer' = function
-  | 1 -> parse_bounded_integer_1
-  | 2 -> parse_bounded_integer_2
-  | 3 -> parse_bounded_integer_3
-  | 4 -> parse_u32
+#set-options "--z3rlimit 16"
+
+let parse_bounded_integer' i = match i with
+  | 1 -> (parse_bounded_integer_1 <: parser (ParserStrong (StrongConstantSize i ConstantSizeTotal)) (bounded_integer i))
+  | 2 -> (parse_bounded_integer_2 <: parser (ParserStrong (StrongConstantSize i ConstantSizeTotal)) (bounded_integer i))
+  | 3 -> (parse_bounded_integer_3 <: parser (ParserStrong (StrongConstantSize i ConstantSizeTotal)) (bounded_integer i))
+  | 4 -> (parse_u32 <: parser (ParserStrong (StrongConstantSize i ConstantSizeTotal)) (bounded_integer i))
+
+#reset-options
