examples/lowparse/LowParse.Impl.VLBytes.Part4.fst
@@ -2,9 +2,9 @@ module LowParse.Impl.VLBytes.Part4
 
 module S = LowParse.Slice
 
-#set-options "--z3rlimit 128"
+#set-options "--z3rlimit 512"
 
-let point_to_vlbytes_contents_correct sz f #b #t p b h len b1 b' =
+let point_to_vlbytes_contents_correct sz f #k #t p b h len b1 b' =
   S.is_concat_is_concat_gen b b1 b'
 
 #reset-options
